\chapter{Matrices}

\section{Symmetric Matrices}

Given a matrix $A_{3x3}$ defined as

$$
A = 
\begin{bmatrix}
a_{11} & a_{12} & a_{13}\\
a_{21} & a_{22} & a_{23}\\
a_{31} & a_{32} & a_{33}
\end{bmatrix}
$$

thus,

$$
A^T = 
\begin{bmatrix}
a_{11} & a_{21} & a_{31}\\
a_{12} & a_{22} & a_{32}\\
a_{13} & a_{23} & a_{33}
\end{bmatrix}
$$

\begin{equation}
    AA^T = 
    \begin{bmatrix}
        (a_{11}a_{11} + a_{12}a_{12} + a_{13}a_{13}) & (a_{11}a_{21} + a_{12}a_{22} + a_{13}a_{23}) & (a_{11}a_{31} + a_{12}a_{32} + a_{13}a_{33})\\
        (a_{21}a_{11} + a_{22}a_{12} + a_{23}a_{13}) & (a_{21}a_{21} + a_{22}a_{22} + a_{23}a_{23}) & (a_{21}a_{31} + a_{22}a_{32} + a_{23}a_{33})\\
        (a_{31}a_{11} + a_{32}a_{12} + a_{33}a_{13}) & (a_{31}a_{21} + a_{32}a_{22} + a_{33}a_{23}) & (a_{31}a_{31} + a_{32}a_{32} + a_{33}a_{33})
    \end{bmatrix}    
\end{equation}

let

$$
K = (a_{11}a_{11} + a_{12}a_{12} + a_{13}a_{13})
$$

$$
L = (a_{11}a_{21} + a_{12}a_{22} + a_{13}a_{23})
$$

$$
H = (a_{11}a_{31} + a_{12}a_{32} + a_{13}a_{33})
$$

$$
M = (a_{21}a_{21} + a_{22}a_{22} + a_{23}a_{23})
$$

$$
N = (a_{21}a_{31} + a_{22}a_{32} + a_{23}a_{33})
$$

$$
G = (a_{31}a_{31} + a_{32}a_{32} + a_{33}a_{33})
$$

then,

\begin{equation}
    AA^T = 
    \begin{bmatrix}
        K & L & H\\
        L & M & N\\
        H & N & G
    \end{bmatrix}    
\end{equation}

and

$$
(AA^T)^T = 
\begin{bmatrix}
    K & L & H\\
    L & M & N\\
    H & N & G
\end{bmatrix}
$$

therefore,

\begin{equation}
    AA^T = (AA^T)^T
\end{equation}

In conclusion, $AA^T$ is a symmetric matrix.

\section{Derivatives}
Given

$$
w = 
\begin{bmatrix}
    w_1\\
    w_2\\
    w_3
\end{bmatrix}
\ \ \ \ A =
\begin{bmatrix}
    a_{11} & a_{12} & a_{13}\\
    a_{21} & a_{22} & a_{23}\\
    a_{31} & a_{32} & a_{33}
\end{bmatrix}
$$

thus,

$$
w^TAw =
[w_1\ w_2\ w_3]
\begin{bmatrix}
    a_{11} & a_{12} & a_{13}\\
    a_{21} & a_{22} & a_{23}\\
    a_{31} & a_{32} & a_{33}
\end{bmatrix}
\begin{bmatrix}
    w_1\\
    w_2\\
    w_3
\end{bmatrix}
$$

$$
w^TAw =
\begin{bmatrix}
    (w_1a_{11} + w_2a_{21} + w_3a_{31}) & (w_1a_{12} + w_2a_{22} + w_3a_{32}) & (w_1a_{13} + w_2a_{23} + w_3a_{33})\\
\end{bmatrix}
\begin{bmatrix}
    w_1\\
    w_2\\
    w_3
\end{bmatrix}
$$

$$
\Leftrightarrow w^TAw =
    (w_1w_1a_{11} + w_1w_2a_{21} + w_1w_3a_{31}) + (w_2w_1a_{12} + w_2w_2a_{22} + w_2w_3a_{32}) + (w_3w_1a_{13} + w_3w_2a_{23} + w_3w_3a_{33})\\
$$

if $A$ is a symmetric matrix, then $a_{21} = a_{12}$, $a_{13} = a_{31}$, $a_{32} = a_{23}$

then,
$$
w^TAw =
    (w_1w_1a_{11} + w_1w_2a_{12} + w_1w_3a_{13}) + (w_2w_1a_{12} + w_2w_2a_{22} + w_2w_3a_{23}) + (w_3w_1a_{13} + w_3w_2a_{23} + w_3w_3a_{33})\\
$$

$$
w^TAw =
    (w_1w_1a_{11} + 2w_1w_2a_{12} + 2w_1w_3a_{13}) + (w_2w_2a_{22} + 2w_2w_3a_{23} +w_3w_3a_{33})\\
$$

$$
\frac{\partial (w^TAw)}{\partial w_1} = \frac{2w_1a_{11} + 2w_2a_{12} + 2w_3a_{13}}{\partial w_1}
$$

$$
\frac{\partial (w^TAw)}{\partial w_2} = \frac{2w_1a_{12} + 2w_2a_{22} + 2w_3a_{23}}{\partial w_2}
$$

$$
\frac{\partial (w^TAw)}{\partial w_3} = \frac{2w_1a_{31} + 2w_2a_{23} + 2w_3a_{33}}{\partial w_3}
$$
in other words,

\begin{equation}
    \frac{\partial w^TAw}{\partial w} = 
    \begin{bmatrix}
        2w_1a_{11} + 2w_2a_{12} + 2w_3a_{13}\\
        2w_1a_{12} + 2w_2a_{22} + 2w_3a_{23}\\
        2w_1a_{31} + 2w_2a_{23} + 2w_3a_{33}
    \end{bmatrix}
\end{equation}


since,

$$
Aw = 
\begin{bmatrix}
    a_{11}w_1 + a_{12}w_2 + a_{13}w_3\\
    a_{21}w_1 + a_{22}w_2 + a_{23}w_3\\
    a_{31}w_1 + a_{32}w_2 + a_{33}w_3
\end{bmatrix}
$$

thus

\begin{equation}
    \frac{\partial w^TAw}{\partial w} = 2Aw
\end{equation}





